theories/ftlr/Lea.v
@@ -7,7 +7,6 @@ From cap_machine.rules Require Import rules_base rules_Lea.
 
 Section fundamental.
   Context {Σ:gFunctors} {memg:memG Σ} {regg:regG Σ}
-          {nainv: logrel_na_invs Σ}
           `{MachineParameters}.
   Notation D := ((leibnizO Word) -n> iPropO Σ).
   Notation R := ((leibnizO Reg) -n> iPropO Σ).
@@ -15,48 +14,50 @@ Section fundamental.
   Implicit Types interp : (D).
 
   Lemma lea_case (r : leibnizO Reg) (p : Perm)
-        (b e a : Addr) (w : Word) (dst : RegName) (r0 : Z + RegName) (P:D):
-    ftlr_instr r p b e a w (Lea dst r0) P.
+        (b e a : Addr) (w : Word) (dst : RegName) (r0 : Z + RegName) (i: CoreN)(P:D):
+    ftlr_instr r p b e a w (Lea dst r0) i P.
   Proof.
-    intros Hp Hsome i Hbae Hi.
-    iIntros "#IH #Hinv #Hinva #Hreg #[Hread Hwrite] Hown Ha HP Hcls HPC Hmap".
+    intros Hp Hsome i' Hbae Hi.
+    iIntros "#IH #Hinv #Hinva #Hreg #[Hread Hwrite] Ha HP Hcls HPC Hmap".
     rewrite delete_insert_delete.
-    iDestruct ((big_sepM_delete _ _ PC) with "[HPC Hmap]") as "Hmap /=";
+    iDestruct ((big_sepM_delete _ _ (i, PC)) with "[HPC Hmap]") as "Hmap /=";
       [apply lookup_insert|rewrite delete_insert_delete;iFrame|]. simpl.
     iApply (wp_lea with "[$Ha $Hmap]"); eauto.
     { by rewrite lookup_insert. }
-    { rewrite /subseteq /map_subseteq /set_subseteq_instance. intros rr _.
-      apply elem_of_gmap_dom. apply lookup_insert_is_Some'; eauto. }
+    { rewrite /regs_of_core /subseteq /map_subseteq /set_subseteq_instance. intros rr ?.
+      apply elem_of_gmap_dom. apply lookup_insert_is_Some'; eauto. set_solver. }
 
     iIntros "!>" (regs' retv). iDestruct 1 as (HSpec) "[Ha Hmap]".
     destruct HSpec as [ * Hdst ? Hz Hoffset HincrPC |].
     { apply incrementPC_Some_inv in HincrPC as (p''&b''&e''&a''& ? & HPC & Z & Hregs').
 
       assert (p'' = p ∧ b'' = b ∧ e'' = e) as (-> & -> & ->).
-      { destruct (decide (PC = dst)); simplify_map_eq; auto. }
+      { destruct (decide (PC = dst)); simplify_map_eq by simplify_pair_eq; auto. }
 
       iApply wp_pure_step_later; auto.
       iMod ("Hcls" with "[HP Ha]");[iExists w;iFrame|iModIntro]. 
       iNext.
-      iApply ("IH" $! regs' with "[%] [] [Hmap] [$Hown]").
+      iApply ("IH" $! _ regs' with "[%] [] [Hmap]").
       { cbn. intros. subst regs'. by repeat (apply lookup_insert_is_Some'; right). }
-      { iIntros (ri v Hri Hvs).
+      { iIntros (j ri v Hri Hvs).
         subst regs'.
         rewrite lookup_insert_ne in Hvs; auto.
-        destruct (decide (ri = dst)).
-        { subst ri.
-          rewrite lookup_insert_ne in Hdst; auto.
+        destruct (decide ((j, ri) = (i, dst))).
+        { simplify_pair_eq.
+          rewrite lookup_insert_ne in Hdst; simplify_pair_eq ; auto.
           rewrite lookup_insert in Hvs; inversion Hvs. simplify_eq.
-          unshelve iSpecialize ("Hreg" $! dst _ _ Hdst); eauto.
+          unshelve iSpecialize ("Hreg" $! i dst _ _ Hdst); eauto.
           iApply interp_weakening; eauto; try solve_addr.
           destruct p0; simpl; auto. }
         { repeat (rewrite lookup_insert_ne in Hvs); auto.
-          iApply "Hreg"; auto. } }
+          iApply "Hreg"; auto.
+          simplify_pair_eq.
+      } simplify_pair_eq. }
       { subst regs'. rewrite insert_insert. iApply "Hmap". }
       iModIntro. rewrite !fixpoint_interp1_eq /=. destruct Hp as [-> | ->];iFrame "Hinv". }
     { iApply wp_pure_step_later; auto.
       iMod ("Hcls" with "[HP Ha]");[iExists w;iFrame|iModIntro]. 
-      iApply wp_value; auto. iNext. iIntros; discriminate. }
+      iApply wp_value; auto. }
   Qed.
 
 End fundamental.
