theories/ftlr/Mov.v
@@ -7,7 +7,6 @@ From cap_machine.rules Require Import rules_base rules_Mov.
 
 Section fundamental.
   Context {Σ:gFunctors} {memg:memG Σ} {regg:regG Σ}
-          {nainv: logrel_na_invs Σ}
           `{MachineParameters}.
 
   Notation D := ((leibnizO Word) -n> iPropO Σ).
@@ -16,75 +15,78 @@ Section fundamental.
   Implicit Types interp : (D).
 
   Lemma mov_case (r : leibnizO Reg) (p : Perm)
-        (b e a : Addr) (w : Word) (dst : RegName) (src : Z + RegName) (P : D):
-    ftlr_instr r p b e a w (Mov dst src) P.
+        (b e a : Addr) (w : Word) (dst : RegName) (src : Z + RegName)
+        (i: CoreN) (P : D):
+    ftlr_instr r p b e a w (Mov dst src) i P.
   Proof.
-    intros Hp Hsome i Hbae Hi.
-    iIntros "#IH #Hinv #Hinva #Hreg #Hread Hown Ha HP Hcls HPC Hmap".
+    intros Hp Hsome i' Hbae Hi.
+    iIntros "#IH #Hinv #Hinva #Hreg #Hread Ha HP Hcls HPC Hmap".
     rewrite delete_insert_delete.
-    iDestruct ((big_sepM_delete _ _ PC) with "[HPC Hmap]") as "Hmap /=";
+    iDestruct ((big_sepM_delete _ _ (i, PC)) with "[HPC Hmap]") as "Hmap /=";
       [apply lookup_insert|rewrite delete_insert_delete;iFrame|]. simpl.
     iApply (wp_Mov with "[$Ha $Hmap]"); eauto.
     { simplify_map_eq; auto. }
-    { rewrite /subseteq /map_subseteq /set_subseteq_instance. intros rr _.
-      apply elem_of_gmap_dom. apply lookup_insert_is_Some'; eauto. }
+    { rewrite /regs_of_core /subseteq /map_subseteq /set_subseteq_instance. intros rr ?.
+      apply elem_of_gmap_dom. apply lookup_insert_is_Some'; eauto. set_solver. }
 
     iIntros "!>" (regs' retv). iDestruct 1 as (HSpec) "[Ha Hmap]".
     destruct HSpec; cycle 1.
     { iApply wp_pure_step_later; auto.
       iMod ("Hcls" with "[Ha HP]"); [iExists w; iFrame|iModIntro]. iNext.
-      iApply wp_value; auto. iIntros; discriminate. }
+      iApply wp_value; auto. }
     { (* TODO: it might be possible to refactor the proof below by using more simplify_map_eq *)
       (* TODO: use incrementPC_inv *)
-      match goal with
-      | H: incrementPC _ = Some _ |- _ => apply incrementPC_Some_inv in H as (p''&b''&e''&a''& ? & HPC & Z & Hregs')
-      end. simplify_map_eq.
+      incrementPC_inv. rename H1 into HPC.
+      (* match goal with *)
+      (* | H: incrementPC _ = Some _ |- _ => apply incrementPC_Some_inv in H as (p''&b''&e''&a''& ? & HPC & Z & Hregs') *)
+      (* end. simplify_map_eq. *)
       iApply wp_pure_step_later; auto.
       iMod ("Hcls" with "[Ha HP]"); [iExists w; iFrame|iModIntro].
       iNext.
       destruct (reg_eq_dec dst PC).
-      { subst dst. rewrite lookup_insert in HPC. inv HPC.
+      { subst dst.
+        rewrite lookup_insert in HPC. inv HPC.
         repeat rewrite insert_insert.
         destruct src; simpl in *; try discriminate.
         destruct (reg_eq_dec PC r0).
-        { subst r0. simplify_map_eq.
-          iApply ("IH" $! r with "[%] [] [Hmap] [$Hown]"); try iClear "IH"; eauto.
+        { subst r0. simplify_map_eq by simplify_pair_eq.
+          iApply ("IH" $! i r with "[%] [] [Hmap]"); try iClear "IH"; eauto.
           iModIntro. rewrite !fixpoint_interp1_eq /=. destruct Hp as [-> | ->]; iFrame "Hinv". }
-        { simplify_map_eq.
-          iDestruct ("Hreg" $! r0 _ _ H0) as "Hr0".
-          destruct (PermFlowsTo RX p'') eqn:Hpft.
-          - iApply ("IH" $! r with "[%] [] [Hmap] [$Hown]"); try iClear "IH"; eauto.
+        { simplify_map_eq by simplify_pair_eq.
+          iDestruct ("Hreg" $! i r0 _ _ H0) as "Hr0".
+          destruct (PermFlowsTo RX x) eqn:Hpft.
+          - iApply ("IH" $! i r with "[%] [] [Hmap]"); try iClear "IH"; eauto.
             + iModIntro.
-              destruct p''; simpl in Hpft; try discriminate; repeat (rewrite fixpoint_interp1_eq); simpl; auto.
-          - iApply (wp_bind (fill [SeqCtx])).
-            iDestruct ((big_sepM_delete _ _ PC) with "Hmap") as "[HPC Hmap]"; [apply lookup_insert|].
-            iApply (wp_notCorrectPC with "HPC"); [eapply not_isCorrectPC_perm; destruct p''; simpl in Hpft; try discriminate; eauto|].
+              destruct x; simpl in Hpft; try discriminate; repeat (rewrite fixpoint_interp1_eq); simpl; auto.
+          - iApply (wp_bind (fill [SeqCtx]) _ _ (_,_) _).
+            iDestruct ((big_sepM_delete _ _ (i, PC)) with "Hmap") as "[HPC Hmap]"; [apply lookup_insert|].
+            iApply (wp_notCorrectPC with "HPC"); [eapply not_isCorrectPC_perm; destruct x; simpl in Hpft; try discriminate; eauto|].
             iNext. iIntros "HPC /=".
             iApply wp_pure_step_later; auto.
             iApply wp_value.
             iNext. iIntros. discriminate. } }
-      { rewrite lookup_insert_ne in HPC; auto.
+      { rewrite lookup_insert_ne in HPC; auto ; simplify_pair_eq.
         rewrite lookup_insert in HPC. inv HPC.
-        iApply ("IH" $! (<[dst:=w0]> _) with "[%] [] [Hmap] [$Hown]"); eauto.
+        iApply ("IH" $! i (<[(i, dst):=w0]> _) with "[%] [] [Hmap]"); eauto.
         - intros; simpl.
           rewrite lookup_insert_is_Some.
-          destruct (reg_eq_dec dst x0); auto; right; split; auto.
+          destruct (reg_eq_dec dst x4); simplify_pair_eq; auto ; right ; split; auto ; simplify_pair_eq.
           rewrite lookup_insert_is_Some.
-          destruct (reg_eq_dec PC x0); auto; right; split; auto.
-       - iIntros (ri v Hri Hvs).
-          destruct (reg_eq_dec ri dst).
-          + subst ri. rewrite lookup_insert in Hvs.
+          destruct (reg_eq_dec PC x4); simplify_pair_eq ; auto ; right; split ; auto ; simplify_pair_eq.
+       - iIntros (j ri v Hri Hvs).
+        destruct (decide ((j, ri) = (i, dst))).
+          + simplify_pair_eq. rewrite lookup_insert in Hvs.
             destruct src; simplify_map_eq.
             * repeat rewrite fixpoint_interp1_eq; auto.
             * destruct (reg_eq_dec PC r0).
               { subst r0.
                 - simplify_map_eq. 
                   rewrite !fixpoint_interp1_eq /=.
-                destruct Hp as [Hp | Hp]; subst p''; try subst g'';
+                destruct Hp as [Hp | Hp]; subst x; try subst g'';
                   (iFrame "Hinv Hexec"). }
-              simplify_map_eq.
-              iDestruct ("Hreg" $! r0 _ _ H0) as "Hr0". auto.
-          + repeat rewrite lookup_insert_ne in Hvs; auto.
+              simplify_map_eq by simplify_pair_eq.
+              iDestruct ("Hreg" $! i r0 _ _ H0) as "Hr0". auto.
+          + repeat rewrite lookup_insert_ne in Hvs; auto ; simplify_pair_eq.
             iApply "Hreg"; auto.
         - iModIntro. rewrite !fixpoint_interp1_eq /=. destruct Hp as [-> | ->]; iFrame "Hinv".
       }
