theories/ftlr/Subseg.v
@@ -8,7 +8,6 @@ From cap_machine.rules Require Import rules_base rules_Subseg.
 
 Section fundamental.
   Context {Σ:gFunctors} {memg:memG Σ} {regg:regG Σ}
-          {nainv: logrel_na_invs Σ}
           `{MachineParameters}.
 
   Notation D := ((leibnizO Word) -n> iPropO Σ).
@@ -31,12 +30,11 @@ Section fundamental.
 
       (b <= b')%a ->
       (e' <= e)%a ->
-      (□ ▷ (∀ a0 a1 a2 a3 a4,
-             full_map a0
-          -∗ (∀ (r1 : RegName) v, ⌜r1 ≠ PC⌝ → ⌜a0 !! r1 = Some v⌝ → (fixpoint interp1) v)
-          -∗ registers_mapsto (<[PC:=WCap a1 a2 a3 a4]> a0)
-          -∗ na_own logrel_nais ⊤
-          -∗ □ (fixpoint interp1) (WCap a1 a2 a3 a4) -∗ interp_conf)) -∗
+      (□ ▷ (∀ i a0 a1 a2 a3 a4,
+             full_map a0 i
+          -∗ (∀ (j: CoreN) (r1 : RegName) v, ⌜r1 ≠ PC⌝ → ⌜a0 !! (j, r1) = Some v⌝ → (fixpoint interp1) v)
+          -∗ registers_mapsto (<[(i, PC):=WCap a1 a2 a3 a4]> a0)
+          -∗ □ (fixpoint interp1) (WCap a1 a2 a3 a4) -∗ interp_conf i)) -∗
       (fixpoint interp1) (WCap p b e a) -∗
       (fixpoint interp1) (WCap p b' e' a).
   Proof.
@@ -46,64 +44,68 @@ Section fundamental.
   Qed.
   
   Lemma subseg_case (r : leibnizO Reg) (p : Perm)
-        (b e a : Addr) (w : Word) (dst : RegName) (r1 r2 : Z + RegName) (P:D):
-    ftlr_instr r p b e a w (Subseg dst r1 r2) P.
+        (b e a : Addr) (w : Word) (dst : RegName) (r1 r2 : Z + RegName)
+        (i:CoreN ) (P:D):
+    ftlr_instr r p b e a w (Subseg dst r1 r2) i P.
   Proof.
-    intros Hp Hsome i Hbae Hi.
-    iIntros "#IH #Hinv #Hinva #Hreg #[Hread Hwrite] Hown Ha HP Hcls HPC Hmap".
+    intros Hp Hsome i' Hbae Hi.
+    iIntros "#IH #Hinv #Hinva #Hreg #[Hread Hwrite] Ha HP Hcls HPC Hmap".
     rewrite delete_insert_delete.
-    iDestruct ((big_sepM_delete _ _ PC) with "[HPC Hmap]") as "Hmap /=";
+    iDestruct ((big_sepM_delete _ _ (i, PC)) with "[HPC Hmap]") as "Hmap /=";
       [apply lookup_insert|rewrite delete_insert_delete;iFrame|]. simpl.
     iApply (wp_Subseg with "[$Ha $Hmap]"); eauto.
     { simplify_map_eq; auto. }
-    { rewrite /subseteq /map_subseteq /set_subseteq_instance. intros rr _.
-      apply elem_of_gmap_dom. apply lookup_insert_is_Some'; eauto. }
+    { rewrite /regs_of_core /subseteq /map_subseteq /set_subseteq_instance. intros rr ?.
+      apply elem_of_gmap_dom. apply lookup_insert_is_Some'; eauto. set_solver. }
 
     iIntros "!>" (regs' retv). iDestruct 1 as (HSpec) "[Ha Hmap]".
     destruct HSpec; cycle 1.
     { iApply wp_pure_step_later; auto.
       iMod ("Hcls" with "[Ha HP]");[iExists w;iFrame|iModIntro;iNext].
-      iApply wp_value; auto. iIntros; discriminate. }
-    { match goal with
-      | H: incrementPC _ = Some _ |- _ => apply incrementPC_Some_inv in H as (p''&b''&e''&a''& ? & HPC & Z & Hregs')
-      end. simplify_map_eq.
+      iApply wp_value; auto. }
+    {
+      apply incrementPC_Some_inv in H5 as (p''&b''&e''&a''& ? & HPC & Z & Hregs').
       iApply wp_pure_step_later; auto.
       iMod ("Hcls" with "[Ha HP]");[iExists w;iFrame|iModIntro;iNext].
       destruct (reg_eq_dec PC dst).
-      { subst dst. repeat rewrite insert_insert in HPC |- *. simplify_map_eq.
-        iApply ("IH" $! r with "[%] [] [Hmap] [$Hown]"); try iClear "IH"; eauto.
-        iModIntro. 
+      { subst dst. repeat (rewrite insert_insert in HPC). simplify_map_eq by simplify_pair_eq.
+        rewrite !insert_insert.
+        iApply ("IH" $! i r with "[%] [] [Hmap]"); try iClear "IH"; eauto.
+        iModIntro.
         generalize (isWithin_implies _ _ _ _ H4). intros [A B].
         destruct (Z_le_dec b'' e'').
         + rewrite !fixpoint_interp1_eq. destruct Hp as [-> | ->].
-          - iSimpl in "Hinv". rewrite (isWithin_finz_seq_between_decomposition b'' e'' b0 e0); auto.
-            iDestruct (big_sepL_app with "Hinv") as "[Hinv1 Hinv2]".
-            iDestruct (big_sepL_app with "Hinv2") as "[Hinv3 Hinv4]".
-            iFrame "#".
-          - iSimpl in "Hinv". rewrite (isWithin_finz_seq_between_decomposition b'' e'' b0 e0); auto.
-            iDestruct (big_sepL_app with "Hinv") as "[Hinv1 Hinv2]".
-            iDestruct (big_sepL_app with "Hinv2") as "[Hinv3 Hinv4]".
-            iFrame "#".
-        + rewrite !fixpoint_interp1_eq /=.
-          (destruct Hp as [-> | ->]; replace (finz.seq_between b'' e'') with (nil: list Addr);
-          try rewrite big_sepL_nil); auto; 
-          unfold finz.seq_between, finz.dist;rewrite Z_to_nat_nonpos //; lia. }
+        - iSimpl in "Hinv". rewrite (isWithin_finz_seq_between_decomposition b'' e'' b0 e0); auto.
+          iDestruct (big_sepL_app with "Hinv") as "[Hinv1 Hinv2]".
+          iDestruct (big_sepL_app with "Hinv2") as "[Hinv3 Hinv4]".
+          iFrame "#".
+        - iSimpl in "Hinv". rewrite (isWithin_finz_seq_between_decomposition b'' e'' b0 e0); auto.
+          iDestruct (big_sepL_app with "Hinv") as "[Hinv1 Hinv2]".
+          iDestruct (big_sepL_app with "Hinv2") as "[Hinv3 Hinv4]".
+          iFrame "#".
+          + rewrite !fixpoint_interp1_eq /=.
+            (destruct Hp as [-> | ->]; replace (finz.seq_between b'' e'') with (nil: list Addr);
+             try rewrite big_sepL_nil); auto;
+            unfold finz.seq_between, finz.dist;rewrite Z_to_nat_nonpos //; lia. }
       { simplify_map_eq.
-        iApply ("IH" $! (<[dst:=_]> _) with "[%] [] [Hmap] [$Hown]"); eauto.
+        iApply ("IH" $! i (<[(i, dst):=_]> _) with "[%] [] [Hmap]"); eauto.
         - intros; simpl.
           rewrite lookup_insert_is_Some.
-          destruct (reg_eq_dec dst x0); auto; right; split; auto.
+          destruct (reg_eq_dec dst x0); simplify_pair_eq ; auto; right; split ; auto; simplify_pair_eq.
           rewrite lookup_insert_is_Some.
-          destruct (reg_eq_dec PC x0); auto; right; split; auto.
-        - iIntros (ri v Hri Hvs).
-          destruct (reg_eq_dec ri dst).
-          + subst ri. rewrite lookup_insert in Hvs. inv Hvs.
-            iDestruct ("Hreg" $! dst _ Hri H0) as "Hdst".
-            generalize (isWithin_implies _ _ _ _ H4). intros [A B]. 
+          destruct (reg_eq_dec PC x0); simplify_pair_eq ; auto; right; split ; auto; simplify_pair_eq.
+        - iIntros (j ri v Hri Hvs).
+          destruct (decide ((j, ri) = (i, dst))).
+          + simplify_pair_eq. rewrite lookup_insert in Hvs. inv Hvs.
+            simplify_map_eq by simplify_pair_eq.
+            iDestruct ("Hreg" $! i dst _ Hri H0) as "Hdst".
+            generalize (isWithin_implies _ _ _ _ H4). intros [A B].
             iApply subseg_interp_preserved; eauto.
-          + repeat rewrite lookup_insert_ne in Hvs; auto.
+          + repeat rewrite lookup_insert_ne in Hvs; auto ; simplify_pair_eq.
             iApply "Hreg"; auto.
-        - rewrite !fixpoint_interp1_eq /=. destruct Hp as [-> | ->];iFrame "Hinv". } }
+        - rewrite !fixpoint_interp1_eq /=.
+            simplify_map_eq by simplify_pair_eq.
+          destruct Hp as [-> | ->]; try iFrame "Hinv". } }
   Qed.
 
 End fundamental.
